theories/syntax/prelude.v
@@ -1,0 +1,7 @@
+Require Import Morphisms Setoid Relation_Definitions core unscoped.
+
+Inductive path_component :=
+| PCProj (n : nat)
+| PCUnwrap.
+
+Definition path := list path_component.
